$$ \omega ^{\omega ^{\omega ^{\epsilon _0 + 1}}} = \omega ^{\epsilon _0 ^{\omega }} = \omega ^{\epsilon _0 ^{1 + \omega }} = \omega ^{\epsilon _0 \epsilon _0 ^{\omega }} = (\omega ^{\epsilon _0}) ^{\epsilon _0 ^{\omega }} = \epsilon _0 ^{\epsilon _0} ^{\omega } $$

$$ \omega ^{\omega ^{\omega ^{\epsilon _0 + 1}}} = $$ 

$$\omega ^{\epsilon _0 ^{\omega }} = $$

$$ \omega ^{\epsilon _0 ^{1 + \omega }} = $$

$$ \omega ^{\epsilon _0 \epsilon _0 ^{\omega }} = $$

$$ (\omega ^{\epsilon _0}) ^{\epsilon _0 ^{\omega }} = $$

$$ \epsilon _0 ^{\epsilon _0} ^{\omega } $$